

Idzorek's method minimisation step: 23/4/20

Substitute $s_k \equiv \frac{1}{\omega_k}$ (scalar)

Solve: $\min_{s_k} \|y - w_k\|^2, s_k > 0.$ y \equiv w_k is the fitted weight vector

$$\text{where } w_k = (\delta \Sigma)^{-1} \underbrace{\left[(\tau \Sigma)^{-1} + s_k p_k^T p_k \right]^{-1}}_{[A + B]^{-1}} \left[(\tau \Sigma)^{-1} \Pi + s_k p_k^T Q_k \right]$$

If B has rank 1 (it does, since p_k is a $1 \times N$ row vector):

$$(A+B)^{-1} = A^{-1} - \frac{1}{1+g} A^{-1} B A^{-1} \quad \text{where } g = \text{tr}(B A^{-1})$$

$$\begin{aligned} \therefore \left[(\tau \Sigma)^{-1} + s_k p_k^T p_k \right]^{-1} &= \tau \Sigma - \frac{1}{1+g} (\tau \Sigma) s_k p_k^T p_k (\tau \Sigma) \\ &= \tau \Sigma - s_k \frac{\tau^2}{1+g} \Sigma p_k^T p_k \Sigma \end{aligned}$$

$$\Rightarrow w_k = (\delta \Sigma)^{-1} \left\{ \Pi + s_k \left[\tau \Sigma p_k^T Q_k - \frac{\tau^2}{1+g} \Sigma p_k^T p_k \Sigma (\tau \Sigma)^{-1} \Pi \right] - s_k^2 \frac{\tau^2}{1+g} \Sigma p_k^T p_k \Sigma p_k^T Q_k \right\}$$

$$= (\delta \Sigma)^{-1} \left\{ \Pi + s_k \tau \left[\Sigma p_k^T Q_k - \frac{1}{1+g} \Sigma p_k^T p_k \Pi \right] - s_k^2 \frac{\tau^2}{1+g} \Sigma p_k^T p_k \Sigma p_k^T Q_k \right\}$$

Dimensions \checkmark

$n \times n$ $n \times 1$ $(n \times n)(n \times 1)(1 \times 1)$ $(n \times n)(n \times 1)(1 \times n)(n \times 1)$ $(n \times n)(n \times 1)(1 \times n)(n \times n)(n \times 1)(1 \times 1)$

$$w_k = (\delta \Sigma)^{-1} \Pi + \frac{s_k \tau}{\delta} \left[p_k^T Q_k - \frac{1}{1+g} p_k^T p_k \Pi \right] - \frac{s_k^2 \tau^2}{\delta(1+g)} p_k^T p_k \Sigma p_k^T Q_k$$

$\therefore w_k = a + b s_k + c s_k^2$ where $a, b, c \in \mathbb{R}^n$.

Let $J(s_k) \equiv \|y - w_k\|^2$ be our cost function.

We want the s_k that minimises J .

$$\begin{aligned} J(s_k) &= (y - w_k)^T (y - w_k) = y^T y - y^T w_k - w_k^T y + w_k^T w_k \\ &= y^T y - y^T (a + b s_k + c s_k^2) - (a^T + b^T s_k + c^T s_k^2) y + w_k^T w_k. \end{aligned}$$

$$\begin{aligned} \frac{\partial J}{\partial s_k} &= -y^T b - 2y^T c s_k - b^T y - 2c^T y s_k + 2b^T b s_k + 4c^T c s_k^3 \\ &\quad + 2a^T b + 4a^T c s_k + 6b^T c s_k^2 \\ &= 2a^T b - y^T b - b^T y + (4a^T c + 2b^T b - 2y^T c - 2c^T y) s_k + 6b^T c s_k^2 + 4c^T c s_k^3 = 0. \end{aligned}$$